c_stubs/tls13_pulse_shims.c
@@ -1,0 +1,18 @@
+#include "tls13_crypto_external.h"
+
+#include <string.h>
+
+void Pulse_Lib_Array_memcpy(
+    size_t len,
+    uint8_t *src,
+    uint8_t *dst,
+    void *src_bytes,
+    void *dst_bytes,
+    void *squash) {
+  (void)src_bytes;
+  (void)dst_bytes;
+  (void)squash;
+  if (len != 0) {
+    memcpy(dst, src, len);
+  }
+}
